\documentclass[11pt]{article}

\usepackage{amsmath}

\title{Sampling Free Boltzmann Machines}
\author{Brian Cheung\\
Jesse Livezey}

\begin{document}
\maketitle

\section{Pretraining with a Stack of RBMs}
As done in \cite{Salakhutdinov2009}, we pretrain our DBM using a stack of modified RBMs.
The probability function for a RBM state is
\begin{equation}
  \label{eq:Prbm}
  P(v,h)=\frac{e^{-E(v,h)}}{Z}=\frac{e^{b_i^vv_i+b_i^hh_i+v_iW_{ij}h_j}}{Z}.
\end{equation}
To learn the weights and biases, we can integrate out the hidden units and use MPF~\cite{Sohl-Dickstein2011} to update the weights.
The hidden units are integrated out as follows:
\begin{equation}
  \label{eq:intouth}
  \begin{split}
    P(v)&=\sum_{h_k=0~\forall k}^1P(v,h)\\
        &=\sum_{h_j=0}^1\frac{e^{b_i^vv_i+b_j^hh_j+v_iW_{ij}h_j}}{Z}\\
        &=e^{b_i^vv_i}\prod_j\sum_{h_j=0}^1e^{(b_j^h+v_iW_{ij})h_j}/Z\\
        &=e^{b_i^vv_i}\prod_j\left(1+e^{(b_j^h+v_iW_{ij})}\right)/Z\\
        &=e^{b_i^vv_i+\sum_j\log\left(1+e^{(b_j^h+v_iW_{ij})}\right)}/Z
  \end{split}
\end{equation}

We can now interpret the terms in the exponent as a new energy for an RBM with hidden weights integrated out.
\begin{equation}
  \label{eq:rbmE}
    E(v) = -b_i^vv_i-\sum_j\log\left(1+e^{(b_j^h+v_iW_{ij})}\right)
\end{equation}

The MPF objective function for this system is:
\begin{equation}
  \label{eq:RBMObj}
    K(\theta) = \frac{\epsilon}{|\mathcal{D}|}\sum_{j\in\mathcal{D}}\sum_{i\in\mathcal{D}_{BF}}\exp{[\tfrac{1}{2}(E_j(\theta)-E_i(\theta))]}
\end{equation}
and the generalized gradient is:
\begin{equation}
  \label{eq:RBMGrad}
    \frac{\partial K}{\partial \theta}(\theta) 
      = \frac{\epsilon}{|\mathcal{D}|}\sum_{j\in\mathcal{D}}\sum_{i\in\mathcal{D}_{BF}}
      \left[\frac{\partial E_j(\theta)}{\partial \theta}-\frac{\partial E_i(\theta)}{\partial \theta} \right]
      \exp{[\tfrac{1}{2}(E_j(\theta)-E_i(\theta))]}.
\end{equation}
We need to calculate the partial derivative of the energy with respect to the weights and biases.
\begin{align}
  \label{eq:dedw}
    \frac{\partial E(v)}{\partial W_{nm}} &= -\frac{e^{b_m^h+v_iW_{im}}v_n}{1+e^{b_m^h+v_iW_{im}}}
      =-v_n\text{sigm}(b_m^h+v_iW_{im})\\
  \label{eq:dedbv}
    \frac{\partial E(v)}{\partial b_n^v} &= -v_n\\
  \label{eq:dedbh}
    \frac{\partial E(v)}{\partial b_n^h} &= -\frac{e^{b_n^h+v_iW_{in}}}{1+e^{b_n^h+v_iW_{in}}}
      =-\text{sigm}(b_n^h+v_iW_{in})
\end{align}

\end{document}
